compiler/core/Translation/Lang/ImpDatatoImpEJson.v
@@ -326,94 +326,9 @@ Section ImpDatatoImpEJson.
                   (imp_data_stmt_to_imp_ejson s2)
       end.
 
-    Section ForRewrite.
-      (* Rewriting functional for into imperative for loop is now isolated *)
-      (* If we want to combine both rewrites into a single pass *)
-      Fixpoint imp_data_stmt_to_imp_ejson_combined (stmt: imp_data_stmt): imp_ejson_stmt :=
-        match stmt with
-        | ImpStmtBlock lv ls =>
-          ImpStmtBlock
-            (map (fun xy => (fst xy,
-                             lift imp_data_expr_to_imp_ejson (snd xy))) lv)
-            (map (imp_data_stmt_to_imp_ejson_combined) ls)
-        | ImpStmtAssign v e =>
-          ImpStmtAssign v (imp_data_expr_to_imp_ejson e)
-        | ImpStmtFor v e s =>
-          let avoid := imp_data_stmt_free_vars stmt ++ imp_data_stmt_bound_vars stmt in
-          let src_id := fresh_var "src" avoid in
-          let avoid := src_id :: avoid in
-          let i_id := fresh_var "i" avoid in
-          let avoid := i_id :: avoid in
-          let src := ImpExprVar src_id in
-          let i := ImpExprVar i_id in
-          ImpStmtBlock
-            [ (src_id, Some (imp_data_expr_to_imp_ejson e)) ]
-            [ ImpStmtForRange
-                i_id
-                (ImpExprConst (ejbigint 0))
-                (* XXX Use src.length - 1, consistent with semantic of 'for i1 to i2 do ... done' loop *)
-                (ImpExprRuntimeCall EJsonRuntimeNatMinus [ ImpExprOp EJsonOpArrayLength [ src ] ; ImpExprConst (ejbigint 1) ])
-                (ImpStmtBlock
-                   [ (v, Some (ImpExprOp EJsonOpArrayAccess [ src; i ])) ]
-                   [ imp_data_stmt_to_imp_ejson_combined s ]) ]
-        | ImpStmtForRange v e1 e2 s =>
-          ImpStmtForRange v
-                          (imp_data_expr_to_imp_ejson e1)
-                          (imp_data_expr_to_imp_ejson e2)
-                          (imp_data_stmt_to_imp_ejson_combined s)
-        | ImpStmtIf e s1 s2 =>
-          ImpStmtIf (imp_data_expr_to_imp_ejson e)
-                    (imp_data_stmt_to_imp_ejson_combined s1)
-                    (imp_data_stmt_to_imp_ejson_combined s2)
-        end.
-
-      Lemma imp_data_stmt_to_imp_ejson_combined_idem (stmt: imp_data_stmt):
-        imp_data_stmt_to_imp_ejson_combined stmt =
-        imp_ejson_stmt_for_rewrite (imp_data_stmt_to_imp_ejson stmt).
-      Proof.
-        (* revert avoid. *)
-        imp_stmt_cases (induction stmt) Case; intros; simpl.
-        + Case "ImpStmtBlock"%string.
-          repeat rewrite map_map.
-          f_equal.
-          assert
-            (Hforall:
-               Forall
-                 (fun stmt : imp_stmt =>
-                    imp_data_stmt_to_imp_ejson_combined (* (map fst el ++ avoid) *) stmt =
-                    imp_ejson_stmt_for_rewrite (* (map fst el ++ avoid) *) (imp_data_stmt_to_imp_ejson stmt)) sl)
-            by
-              (apply (@Forall_impl
-                        imp_stmt
-                        (fun stmt : imp_stmt =>
-                           forall avoid : list string,
-                             imp_data_stmt_to_imp_ejson_combined (* avoid *) stmt =
-                             imp_ejson_stmt_for_rewrite (* avoid *) (imp_data_stmt_to_imp_ejson stmt))
-                        (fun stmt : imp_stmt =>
-                           imp_data_stmt_to_imp_ejson_combined (* (map fst el ++ avoid) *) stmt =
-                           imp_ejson_stmt_for_rewrite (* (map fst el ++ avoid) *) (imp_data_stmt_to_imp_ejson stmt)));
-               try assumption; intros; apply H0); clear H.
-          apply (map_eq Hforall).
-        + Case "ImpStmtAssign"%string.
-          reflexivity.
-        + Case "ImpStmtFor"%string.
-          repeat f_equal.
-          rewrite IHstmt.
-          reflexivity.
-        + Case "ImpStmtForRange"%string.
-          rewrite IHstmt.
-          reflexivity.
-        + Case "ImpStmtIf"%string.
-          repeat f_equal.
-          apply IHstmt1.
-          apply IHstmt2.
-      Qed.
-
-    End ForRewrite.
-
     Definition imp_data_function_to_imp_ejson (f:imp_data_function) : imp_ejson_function :=
       match f with
-      | ImpFun v s ret => ImpFun v (imp_data_stmt_to_imp_ejson(* _combined [v] *) s) ret
+      | ImpFun v s ret => ImpFun v (imp_data_stmt_to_imp_ejson s) ret
       end.
 
     Definition imp_data_to_imp_ejson (i:imp_data) : imp_ejson :=
@@ -1315,21 +1230,6 @@ reflexivity.
         match_destr.
     Qed.
 
-    Section CorrectnessForRewrite.
-      Lemma imp_data_stmt_to_imp_ejson_stmt_combined_correct (σ:pd_bindings) (stmt:imp_data_stmt) :
-        forall avoid,
-          unlift_result_env (imp_data_stmt_eval h stmt σ) =
-          imp_ejson_stmt_eval h (imp_data_stmt_to_imp_ejson_combined avoid stmt) (lift_pd_bindings σ).
-      Proof.
-        intros.
-        rewrite imp_data_stmt_to_imp_ejson_combined_idem; simpl.
-        rewrite imp_data_stmt_to_imp_ejson_stmt_correct.
-        rewrite (imp_ejson_stmt_for_rewrite_correct h (lift_pd_bindings σ) _ avoid).
-        reflexivity.
-      Qed.
-
-    End CorrectnessForRewrite.
-    
     Lemma imp_data_function_to_imp_ejson_function_correct (d:data) (f:imp_data_function) :
       imp_data_function_eval h f d =
       lift ejson_to_data (imp_ejson_function_eval h (imp_data_function_to_imp_ejson f) (data_to_ejson d)).
